src/Arithmetic/Inv.v
@@ -1,0 +1,1223 @@
+Require Import Coq.Bool.Bool.
+Require Import Coq.ZArith.ZArith.
+Require Import Coq.Lists.List.
+Require Import Coq.nsatz.Nsatz.
+Require Import Coq.micromega.Lia.
+Require Import Crypto.Arithmetic.UniformWeight.
+Require Import Crypto.Arithmetic.Saturated.
+Require Import Crypto.Arithmetic.Core.
+Require Import Crypto.Arithmetic.WordByWordMontgomery.
+
+Require Import Crypto.Util.LetIn.
+Require Import Crypto.Util.ListUtil.
+Require Import Crypto.Util.ZUtil.Notations.
+Require Import Crypto.Arithmetic.Partition.
+Require Import Crypto.Util.Decidable.
+Require Import Crypto.Util.ZUtil.Definitions.
+Require Import Crypto.Util.ZUtil.TruncatingShiftl.
+Require Import Crypto.Util.ZUtil.Modulo.
+Require Import Crypto.Util.ZUtil.Testbit.
+Require Import Crypto.Util.ZUtil.Shift.
+Require Import Crypto.Util.ZUtil.Div.
+Require Import Crypto.Util.ZUtil.Lor.
+Require Import Crypto.Util.ZUtil.Land.
+Require Import Crypto.Util.ZUtil.ArithmeticShiftr.
+
+Import Positional.
+Import ListNotations.
+Import Definitions.
+
+(** An implementation of the divsteps2 algorithm from "Fast constant-time gcd computation and modular inversion."
+   by D. J. Bernstein et al. See the file inversion-c/readme.txt for generation of C-code.
+   For a C-implementation using this generated code to implement modular inversion, see inversion-c/test-inversion.c. **)
+
+Local Coercion Z.of_nat : nat >-> Z.
+
+Local Open Scope Z_scope.
+
+(************* *)
+(**Definitions *)
+(************* *)
+
+(*twos complement evaluation *)
+Notation twosc m a :=
+  (if ((a mod 2 ^ m) <? 2 ^ (m - 1)) then a mod 2 ^ m else a mod 2 ^ m - 2 ^ m).
+
+(*Custom evaluation function for multi-limbg twos complement *)
+Definition eval_twosc machine_wordsize n f :=
+  twosc (machine_wordsize * Z.of_nat n) (eval (uweight machine_wordsize) n f).
+
+(*Saturated addition of multi-limb integers *)
+Local Definition sat_add machine_wordsize n f g :=
+  fst (Rows.add (uweight machine_wordsize) n f g).
+
+(*Saturated (logical) right shift *)
+Definition sat_shiftr machine_wordsize n f :=
+  (map
+    (fun i =>
+       Z.lor (Z.shiftr (nth_default 0 f i) 1)
+             (Z.truncating_shiftl machine_wordsize
+                           (nth_default 0 f (S i))
+                           (machine_wordsize - 1)))
+    (seq 0 (n - 1))) ++ [(nth_default 0 f (n - 1)) >> 1].
+
+(* arithmetic right shift of saturated multi-limb integers *)
+Definition sat_arithmetic_shiftr machine_wordsize n f :=
+  (map
+     (fun i =>
+        ((nth_default 0 f i) >> 1) |' (Z.truncating_shiftl machine_wordsize
+                                                    (nth_default 0 f (i + 1))
+                                                    (machine_wordsize - 1)))
+     (seq 0 (n - 1)))
+    ++ [Z.arithmetic_shiftr machine_wordsize (nth_default 0 f (n - 1))].
+
+(* Multi-limb parity check *)
+Definition sat_mod2 f :=
+  nth_default 0 f 0 mod 2.
+
+Local Notation sat_one machine_wordsize n := (encode_no_reduce (uweight machine_wordsize) n 1).
+
+Definition sat_opp machine_wordsize n f :=
+  sat_add machine_wordsize n
+          (sat_one machine_wordsize n)
+          (map (fun i => Z.lnot_modulo i (2^machine_wordsize)) f).
+
+Definition sat_zero n :=
+  repeat 0 n.
+  (* encode_no_reduce (uweight machine_wordsize) n 0. *)
+
+(************************************************* *)
+(**Lemmas about the twos complement representation *)
+(************************************************* *)
+
+Lemma twosc_one m (Hm : 1 < m) :
+  twosc m 1 = 1.
+Proof.
+  assert (1 < 2 ^ m) by (apply Zpow_facts.Zpower_gt_1; lia).
+  assert (1 < 2 ^ (m - 1)) by (apply Zpow_facts.Zpower_gt_1; lia).
+  apply Z.ltb_lt in H0. rewrite Z.mod_small, H0; lia. Qed.
+
+Lemma twosc_zero m (Hm : 0 < m):
+  twosc m 0 = 0.
+Proof.
+  assert (0 <? 2 ^ (m - 1) = true).
+  apply Z.ltb_lt; auto with zarith.
+  rewrite Z.mod_0_l by auto with zarith.
+  rewrite H; reflexivity. Qed.
+
+Lemma twosc_mod a m (Hm : 0 < m) :
+  twosc m (a mod 2 ^ m) = twosc m a.
+Proof. rewrite Z.mod_mod; try apply Z.pow_nonzero; lia. Qed.
+
+Lemma twosc_odd m a (Hm : 0 < m) : Z.odd (twosc m a) = Z.odd a.
+Proof.
+  destruct (a mod 2 ^m <? 2 ^ (m - 1));
+    simpl;
+    [ | unfold Z.sub; rewrite Z.odd_add_even];
+    rewrite ?Zodd_mod, <- ?(Znumtheory.Zmod_div_mod);
+    try (apply Z.pow_pos_nonneg; lia);
+    try (apply Zpow_facts.Zpower_divide; lia);
+    try reflexivity.
+  apply Z.even_spec. rewrite Z.even_opp, Z.even_pow; try lia; reflexivity. Qed.
+
+Lemma twosc_mod2 m a (Hm : 0 < m) : twosc m a mod 2 = a mod 2.
+Proof. rewrite Zmod_odd, twosc_odd, <- Zmod_odd by lia. reflexivity. Qed.
+
+Lemma twosc_bounds a m (Hm : 0 < m) :
+  - 2 ^ (m - 1) <= twosc m a < 2 ^ (m - 1).
+Proof.
+  assert (0 < 2 ^ m) by (apply Z.pow_pos_nonneg; lia).
+  assert (2 ^ m = 2 * 2 ^ (m - 1))
+    by (rewrite Pow.Z.pow_mul_base, Z.sub_simpl_r; lia).
+  pose proof (Z.mod_pos_bound a (2 ^ m) H).
+  destruct (a mod 2 ^ m <? 2 ^ (m - 1)) eqn:E.
+  - rewrite Z.ltb_lt in E; lia.
+  - apply Z.ltb_ge in E; lia. Qed.
+
+(*********************************************************************** *)
+(**Section for small independent lemmas which do not fit anywhere else   *)
+(*********************************************************************** *)
+
+Lemma app_split {A} (a b c d : list A) : a = c -> b = d -> a ++ b = c ++ d.
+Proof. now intros; subst. Qed.
+
+Lemma eval_bound machine_wordsize n f
+      (mw0 : 0 < machine_wordsize)
+      (Hz : forall z, In z f -> 0 <= z < 2^machine_wordsize)
+      (Hf : length f = n) :
+  0 <= eval (uweight machine_wordsize) n f < 2 ^ (machine_wordsize * n).
+Proof.
+  generalize dependent n; induction f; intros; subst; simpl in *.
+  - rewrite eval0, Z.mul_0_r, Z.pow_0_r; lia.
+  - rewrite eval_cons, uweight_eval_shift, uweight_0, uweight_eq_alt' by lia.
+    assert (0 <= 2 ^ machine_wordsize) by (apply Z.pow_nonneg; lia).
+    specialize (IHf (fun z H => Hz z (or_intror H)) (length f) eq_refl).
+    specialize (Hz a (or_introl eq_refl)).
+    split; ring_simplify; rewrite Z.mul_1_r.
+    + nia.
+    + replace (machine_wordsize * Z.pos (Pos.of_succ_nat (length f))) with
+        (machine_wordsize + machine_wordsize * Z.of_nat (length f)) by nia.
+      rewrite Z.pow_add_r; nia. Qed.
+
+Lemma mod_less_than_half_iff_not_neg_mod_less a m
+        (Hm : 0 < m)
+        (Ha1 : a mod 2 ^ m <> 2 ^ (m - 1))
+        (Ha2 : a mod 2 ^ m <> 0) :
+  (a mod 2 ^ m <? 2 ^ (m - 1)) = negb ((- a) mod 2 ^ m <? 2 ^ (m - 1)).
+Proof.
+  assert (0 < 2 ^ m) by (apply Z.pow_pos_nonneg; lia).
+  assert (a mod 2 ^ m + (- a mod 2 ^ m) = 2 * 2 ^ (m - 1)) by
+      (rewrite !Zmod_eq, Z_div_nz_opp_full, Pow.Z.pow_mul_base, Z.sub_simpl_r by lia; ring).
+  destruct (a mod 2 ^ m <? 2 ^ (m - 1)) eqn:E1;
+    destruct (- a mod 2 ^ m <? 2 ^ (m - 1)) eqn:E2;
+    rewrite ?Z.ltb_lt, ?Z.ltb_ge in *; try reflexivity; lia. Qed.
+
+(****************************************************************************** *)
+(**Section for lemma relating to bitwise operations and the Z.testbits function *)
+(****************************************************************************** *)
+
+Lemma eval_testbit machine_wordsize n f m
+      (Hz : forall z, In z f -> 0 <= z < 2^machine_wordsize)
+      (mw0 : 0 < machine_wordsize)
+      (Hf : length f = n)
+      (Hm : 0 <= m) :
+  Z.testbit (eval (uweight machine_wordsize) n f) m =
+  Z.testbit (nth_default 0 f (Z.abs_nat (m / machine_wordsize))) (m mod machine_wordsize).
+Proof.
+  generalize dependent n. generalize dependent m. induction f; intros; simpl in *; subst.
+  - rewrite ListUtil.nth_default_nil, eval0, !Z.testbit_0_l; reflexivity.
+  - rewrite eval_cons, uweight_eval_shift by lia.
+    rewrite uweight_0, uweight_eq_alt', Z.mul_1_l, Z.mul_1_r, Z.mul_comm, <- Z.shiftl_mul_pow2, Shift.Z.testbit_add_shiftl_full; try lia.
+    destruct (m <? machine_wordsize) eqn:E.
+    + rewrite Z.ltb_lt in E; rewrite Z.div_small by lia.
+      rewrite ListUtil.nth_default_cons, Z.mod_small by lia. reflexivity.
+    + rewrite Z.ltb_ge in E; rewrite IHf; try lia.
+      replace (Z.abs_nat (m / machine_wordsize)) with
+          (S (Z.abs_nat ((m - machine_wordsize) / machine_wordsize))).
+      rewrite ListUtil.nth_default_cons_S, PullPush.Z.sub_mod_r, Z_mod_same_full, Z.sub_0_r; reflexivity.
+      rewrite <- Zabs2Nat.inj_succ_abs, Z.abs_eq.
+      replace machine_wordsize with (1 * machine_wordsize) at 1 by ring.
+      rewrite Div.Z.div_sub, Z.sub_1_r, Z.succ_pred; lia.
+      apply Div.Z.div_nonneg; lia.
+      intros; specialize (Hz z); tauto.
+    + specialize (Hz a (or_introl eq_refl)); lia. Qed.
+
+(**************************************************** *)
+(**Functional correctness of multi-limb logical shift *)
+(**************************************************** *)
+
+Lemma eval_sat_shiftr machine_wordsize n f
+      (mw0 : 0 < machine_wordsize)
+      (Hf : length f = n)
+      (Hz : forall z, In z f -> 0 <= z < 2^machine_wordsize) :
+  eval (uweight machine_wordsize) n (sat_shiftr machine_wordsize n f) =
+  eval (uweight machine_wordsize) n f >> 1.
+Proof.
+  generalize dependent n. induction f; intros; subst.
+  - unfold sat_shiftr; simpl; rewrite eval0; reflexivity.
+  - unfold sat_shiftr; simpl.
+    rewrite eval_cons, uweight_eval_shift; try lia.
+    destruct f; simpl in *.
+    + rewrite
+        eval_cons, uweight_0, eval0, ListUtil.nth_default_cons, uweight_eq_alt',
+        Z.mul_0_r, !Z.add_0_r, !Z.mul_1_l; reflexivity.
+    + rewrite eval_cons, uweight_eval_shift;
+        try (rewrite ?length_snoc, ?map_length, ?seq_length; lia).
+      replace ((map _ _) ++ _) with (sat_shiftr machine_wordsize (S (length f)) (z :: f)).
+      * rewrite IHf; try (intros; try apply Hz; tauto).
+        rewrite uweight_0, ListUtil.nth_default_cons_S, uweight_eq_alt'.
+        rewrite !ListUtil.nth_default_cons, !Z.mul_1_l, !Z.mul_1_r.
+        rewrite <- !Z.div2_spec, !Z.div2_div, Z.div2_split by lia.
+        rewrite eval_cons at 2 by reflexivity.
+        rewrite uweight_eval_shift, uweight_0, uweight_eq_alt, Z.pow_1_r by lia.
+        rewrite PullPush.Z.add_mod_r, PullPush.Z.mul_mod_l.
+        replace 2 with (2 ^ 1) at 7 by trivial.
+        rewrite Modulo.Z.mod_same_pow, Z.mul_0_l by lia. ring_simplify.
+        rewrite Z.mul_1_l, Z.add_0_r, Z.truncating_shiftl_mod by lia. rewrite Z.lor_add; try ring.
+        destruct (Z.odd z) eqn:E; rewrite Zmod_odd, E.
+        ** specialize (Hz a (or_introl eq_refl)).
+           rewrite Z.mul_1_r, Z.land_div2; rewrite ?Z.sub_simpl_r; lia.
+        ** now rewrite Z.mul_0_r, Z.land_0_r.
+      * unfold sat_shiftr. replace (S (length f) - 1)%nat with (length f) by omega.
+        apply app_split.
+        ** apply map_seq_ext; intros; try lia.
+           rewrite Nat.sub_0_r, Nat.add_1_r.
+           rewrite !(ListUtil.nth_default_cons_S _ a); reflexivity.
+        ** now rewrite ListUtil.nth_default_cons_S. Qed.
+
+(*********************************************************************************** *)
+(**Section for properties of the multi-limb addtion including functional correctness *)
+(*********************************************************************************** *)
+
+Lemma eval_sat_add machine_wordsize n f g (mw0 : 0 < machine_wordsize) (Hf : length f = n) (Hg : length g = n) :
+  eval (uweight machine_wordsize) n (sat_add machine_wordsize n f g) =
+  (eval (uweight machine_wordsize) n f + eval (uweight machine_wordsize) n g) mod (2^(machine_wordsize * n)).
+Proof.
+  unfold sat_add.
+  rewrite Rows.add_partitions;
+    rewrite ?eval_partition; try assumption; try apply (uwprops machine_wordsize mw0).
+  rewrite uweight_eq_alt'; reflexivity. Qed.
+
+Lemma length_sat_add machine_wordsize n f g
+      (mw0 : 0 < machine_wordsize)
+      (Hf : length f = n)
+      (Hg : length g = n) :
+  length (sat_add machine_wordsize n f g) = n.
+Proof.
+  unfold sat_add, Rows.add.
+  autorewrite with distr_length. reflexivity.
+  apply (uwprops machine_wordsize mw0).
+  intros row H; destruct H as [|[H|[]]]; subst; auto. Qed.
+
+Hint Rewrite length_sat_add : length_distr.
+
+Lemma sat_add_bounds machine_wordsize n f g
+      (mw0 : 0 < machine_wordsize)
+      (Hf : length f = n)
+      (Hg : length g = n) :
+  forall z, In z (sat_add machine_wordsize n f g) -> 0 <= z < 2 ^ machine_wordsize.
+Proof.
+  intros. unfold sat_add in *.
+  rewrite Rows.add_partitions in *; auto.
+  unfold Partition.partition in H.
+  apply ListAux.in_map_inv in H.
+  destruct H as [a [H]].
+  rewrite H0, !uweight_eq_alt; try lia.
+  split.
+  - apply Z.div_le_lower_bound;
+      ring_simplify; try apply Z.mod_pos_bound;
+        apply Z.pow_pos_nonneg; try lia; apply Z.pow_pos_nonneg; lia.
+  - apply Z.div_lt_upper_bound.
+    apply Z.pow_pos_nonneg; try lia; apply Z.pow_pos_nonneg; lia.
+    replace ((_ ^ _) ^ _ * _) with ((2 ^ machine_wordsize) ^ Z.of_nat (S a)).
+    apply Z.mod_pos_bound; apply Z.pow_pos_nonneg; try lia; apply Z.pow_pos_nonneg; lia.
+    rewrite Z.mul_comm, Pow.Z.pow_mul_base; 
+    try (replace (Z.of_nat (S a)) with ((Z.of_nat a + 1)) by lia; lia).
+  - apply (uwprops machine_wordsize mw0). Qed.
+
+(********************************************************* *)
+(**Section on properties of sat_mod2 including correctness *)
+(********************************************************* *)
+
+Lemma sat_mod2_cons a f : sat_mod2 (a :: f) = a mod 2.
+Proof. unfold sat_mod2. now rewrite ListUtil.nth_default_cons. Qed.
+
+Lemma eval_sat_mod2 machine_wordsize n f
+      (Hf : length f = n)
+      (Hmw : 0 < machine_wordsize) :
+  (eval (uweight machine_wordsize) n f) mod 2 = sat_mod2 f.
+Proof.
+  generalize dependent Hf. generalize dependent n.
+  induction f; intros; simpl in *; subst.
+  - unfold sat_mod2. rewrite eval0; reflexivity.
+  - rewrite eval_cons by trivial. rewrite uweight_eval_shift by lia.
+    rewrite <- Zplus_mod_idemp_r, <- Zmult_mod_idemp_r, IHf by reflexivity.
+    unfold uweight, ModOps.weight; simpl.
+    rewrite Z.mul_0_r, Z.mul_1_r, !Zdiv_1_r, !Z.opp_involutive, !Z.pow_0_r, Z.mul_1_l.
+    rewrite <- Zmult_mod_idemp_l, PullPush.Z.mod_pow_full, Z_mod_same_full, Z.pow_0_l by assumption.
+    rewrite Zmod_0_l, Z.add_0_r; reflexivity. Qed.
+
+(*********************************************************************** *)
+(**Section for properties of sat_arithmetic_shiftr including correctness *)
+(*********************************************************************** *)
+
+Lemma eval_sat_arithmetic_shiftr machine_wordsize n f
+      (mw0 : 0 < machine_wordsize)
+      (Hz : forall z, In z f -> 0 <= z < 2^machine_wordsize)
+      (Hf : length f = n) :
+  eval (uweight machine_wordsize) n (sat_arithmetic_shiftr machine_wordsize n f) =
+  Z.arithmetic_shiftr (machine_wordsize * n) (eval (uweight machine_wordsize) n f).
+Proof.
+  generalize dependent n.
+  induction f as [|z f IHf]; intros; subst.
+  - rewrite !eval0; reflexivity.
+  - destruct f.
+    + cbn; rewrite uweight_0, !Z.mul_1_r, !Z.mul_1_l, !Z.add_0_r; reflexivity.
+    + unfold sat_arithmetic_shiftr; simpl.
+      rewrite eval_cons, !uweight_eval_shift by (try lia; autorewrite with distr_length; reflexivity).
+      replace (map _ _ ++ _) with (sat_arithmetic_shiftr machine_wordsize (S (length f)) (z0 :: f)).
+      rewrite IHf; try reflexivity.
+
+      unfold Z.arithmetic_shiftr; rewrite !Z.land_pow2_testbit, !eval_testbit; try tauto; try nia; simpl.
+      replace (Z.abs_nat ((machine_wordsize * Z.pos (Pos.succ (Pos.of_succ_nat (length f))) - 1) / machine_wordsize)) with
+          (S (Z.abs_nat ((machine_wordsize * Z.pos (Pos.of_succ_nat (length f)) - 1) / machine_wordsize))).
+      rewrite !ListUtil.nth_default_cons_S, !ListUtil.nth_default_cons by lia.
+
+      unfold Z.sub.
+      rewrite !Modulo.Z.mod_add_l', uweight_0, uweight_eq_alt', !Z.mul_1_l, Z.mul_1_r, Z.truncating_shiftl_mod by lia.
+      destruct (Z.testbit
+      (nth_default 0 (z0 :: f)
+         (Z.abs_nat
+            ((machine_wordsize * Z.pos (Pos.of_succ_nat (length f)) + - (1)) /
+             machine_wordsize)))
+      ((- (1)) mod machine_wordsize)) eqn:E.
+      * rewrite <- !Z.div2_spec, !Z.div2_div, !Z.lor_add; ring_simplify.
+        rewrite (eval_cons _ (S _)), uweight_eval_shift by (try reflexivity; lia).
+        rewrite uweight_0, uweight_eq_alt', !Z.mul_1_l, Z.mul_1_r, Z.div2_split, <- Z.pow_add_r by nia.
+        rewrite eval_sat_mod2 by (try reflexivity; lia). unfold sat_mod2.
+        rewrite ListUtil.nth_default_cons.
+        replace (machine_wordsize + (_ + _)) with
+            (machine_wordsize * Z.pos (Pos.succ (Pos.of_succ_nat (length f))) + - (1)) by lia; ring.
+
+        rewrite Z.land_comm, Z.land_pow2_small; try lia.
+        split.
+        apply Div.Z.div_nonneg; try lia.
+           assert (0 <= eval (uweight machine_wordsize) (S (S (length f))) (z :: z0 :: f)).
+           { apply eval_bound; try lia. intros; apply Hz; simpl; tauto. reflexivity. }
+           specialize (Hz z (or_introl eq_refl)); nia.
+        apply Div.Z.div_lt_upper_bound'; try lia.
+           rewrite Z.mul_comm, Pow.Z.pow_mul_base by nia.
+        simpl; rewrite <- Z.add_assoc, Z.add_0_r.
+        apply eval_bound; try lia; tauto.
+
+        rewrite Z.land_comm, Z.land_pow2_small; try lia.
+        split.
+        apply Div.Z.div_nonneg; try lia.
+        apply eval_bound; try lia. intros; apply Hz; simpl; tauto. reflexivity.
+
+        apply Div.Z.div_lt_upper_bound'; try lia.
+        rewrite Z.mul_comm, Pow.Z.pow_mul_base; try nia. rewrite <- Z.add_assoc, Z.add_0_r.
+        apply eval_bound; try lia. intros; apply Hz; simpl; tauto. reflexivity.
+
+        rewrite Zmod_odd.
+        specialize (Hz z (or_introl eq_refl)).
+        destruct (Z.odd z0).
+        ** rewrite Z.mul_1_r, Z.land_pow2_small; try lia. split.
+           apply Div.Z.div_nonneg; lia.
+           apply Div.Z.div_lt_upper_bound'; try lia.
+           rewrite Z.mul_comm, Pow.Z.pow_mul_base, Z.sub_simpl_r; lia.
+        ** rewrite Z.mul_0_r, Z.land_0_r; reflexivity.
+      * rewrite !Z.lor_0_l, (eval_cons _ (S _)), uweight_eval_shift; try lia; try reflexivity.
+        rewrite uweight_0, uweight_eq_alt', Z.mul_1_l, Z.mul_1_r.
+        rewrite <- !Z.div2_spec, !Z.div2_div, Z.div2_split by lia.
+        rewrite eval_sat_mod2, sat_mod2_cons, Z.lor_add; try lia ; try reflexivity.
+        rewrite Zmod_odd. specialize (Hz z (or_introl eq_refl)).
+        destruct (Z.odd z0).
+        ** rewrite Z.mul_1_r, Z.land_pow2_small; try lia.
+           split.
+           apply Div.Z.div_nonneg; lia.
+           apply Div.Z.div_lt_upper_bound'; [lia|].
+           rewrite Z.mul_comm, Pow.Z.pow_mul_base, Z.sub_simpl_r; lia.
+        ** rewrite Z.mul_0_r, Z.land_0_r; reflexivity.
+      * rewrite <- Zabs2Nat.inj_succ.
+        apply f_equal.
+        rewrite <- Z.add_1_r.
+        unfold Z.sub.
+        rewrite !Div.Z.div_add_l'; lia.
+        set (x := Pos.of_succ_nat (length f)).
+        set (a := machine_wordsize). apply Div.Z.div_nonneg; nia.
+      * intros; apply Hz; simpl in *; tauto.
+      * intros; apply Hz; simpl in *; tauto.
+      * unfold sat_arithmetic_shiftr.
+        replace (S (length f) - 1)%nat with (length f) by lia.
+        rewrite ListUtil.nth_default_cons_S.
+        apply f_equal2; [|reflexivity].
+        apply map_seq_ext; [|lia].
+        intros; simpl; rewrite !Nat.add_1_r, !(ListUtil.nth_default_cons_S _ z); reflexivity. Qed.
+
+(************************************ *)
+(**Properties of sat_one and sat_zero *)
+(************************************ *)
+
+Lemma length_sat_one machine_wordsize n :
+  length (sat_one machine_wordsize n) = n.
+Proof. auto with distr_length. Qed.
+
+Lemma length_sat_zero n :
+  length (sat_zero n) = n.
+Proof. auto with distr_length. Qed.
+
+Lemma eval_sat_zero machine_wordsize n (mw : 0 < machine_wordsize):
+  eval (uweight machine_wordsize) n (sat_zero n) = 0.
+Proof.
+  unfold sat_zero; induction n.
+  - reflexivity.
+  - simpl; rewrite eval_cons, uweight_eval_shift, uweight_0, IHn;
+      auto with distr_length; lia. Qed.
+
+(******************************************************** *)
+(**Properties of sat_opp including functional correctness *)
+(******************************************************** *)
+
+Lemma length_sat_opp machine_wordsize n f
+      (mw0 : 0 < machine_wordsize)
+      (Hf : length f = n) :
+  length (sat_opp machine_wordsize n f) = n.
+Proof. unfold sat_opp; rewrite length_sat_add; auto with distr_length; lia. Qed.
+
+Hint Rewrite length_sat_opp : distr_length.
+
+Lemma eval_sat_opp machine_wordsize n f
+      (mw0 : 0 < machine_wordsize)
+      (Hz : forall z, In z f -> 0 <= z < 2^machine_wordsize)
+      (Hf : length f = n) :
+  eval (uweight machine_wordsize) n (sat_opp machine_wordsize n f) =
+  (- eval (uweight machine_wordsize) n f) mod (2^(machine_wordsize * n)).
+Proof.
+  assert (2 ^ machine_wordsize <> 0) by (apply Z.pow_nonzero; lia).
+  assert (2 ^ (machine_wordsize * Z.of_nat (length f)) <> 0) by (apply Z.pow_nonzero; nia).
+
+  symmetry. unfold sat_opp.
+  rewrite eval_sat_add by distr_length.
+  generalize dependent n. induction f; intros.
+  - simpl in *; rewrite <- Hf; rewrite eval0; rewrite !Zmod_0_l; reflexivity.
+  - simpl in *. subst.
+    assert (2 ^ (machine_wordsize * Z.of_nat (length f)) <> 0) by (apply Z.pow_nonzero; nia).
+
+    rewrite !eval_cons, uweight_0, !uweight_eval_shift, uweight_eq_alt' by distr_length.
+    rewrite !Z.mul_1_l, !Z.mul_1_r, Z.opp_add_distr, Zopp_mult_distr_r, <- Z.add_mod_idemp_r by distr_length.
+    symmetry. rewrite Z.add_assoc, <- Z.add_mod_idemp_r; try (rewrite Zpos_P_of_succ_nat in H0; rewrite Nat2Z.inj_succ; assumption). 
+    replace (2 ^ (machine_wordsize * Z.of_nat (S (length f)))) with
+        ((2 ^ machine_wordsize) * (2 ^ (machine_wordsize * Z.of_nat (length f)))).
+    rewrite !Z.mul_mod_distr_l; try lia.
+    unfold Z.lnot_modulo. rewrite Lnot.Z.lnot_equiv. unfold Z.pred.
+    rewrite IHf; try lia.
+    destruct (length f) eqn:E.
+    + rewrite !eval0.
+      rewrite !Z.mul_0_r, !Z.mul_1_r, !Z.add_0_r.
+      replace (-a + -1) with (- (a + 1)) by ring.
+      rewrite eval_encode_no_reduce.
+      rewrite Z.mod_opp_small.
+      replace (1 + (2 ^ machine_wordsize - (a + 1))) with
+          (-a + 2 ^ machine_wordsize) by ring.
+      rewrite <- Z.add_mod_idemp_r.
+      rewrite Z_mod_same_full. rewrite Z.add_0_r. reflexivity.
+      apply Z.pow_nonzero. omega. lia.
+      specialize (Hz a (or_introl eq_refl)). lia.
+      rewrite uweight_0. reflexivity.
+      intro; symmetry; apply Z.lt_neq;
+        apply (weight_positive (uwprops machine_wordsize mw0)). omega.
+      intros; symmetry; apply Z.lt_neq;
+        apply (weight_divides (uwprops machine_wordsize mw0)).
+    + rewrite !eval_encode_no_reduce in *; try lia; try apply uweight_0.
+      rewrite <- Z.mul_mod_distr_l, Z.add_mod_idemp_r; try nia.
+      symmetry.
+      rewrite <- Z.mul_mod_distr_l, Z.add_mod_idemp_r, Z.mul_add_distr_l, Z.mul_1_r; try nia.
+      replace (-a + -1) with (- (a + 1)) by ring.
+      rewrite Z.mod_opp_small.
+      unfold Z.lnot_modulo.
+      rewrite Z.add_assoc.
+      replace (1 + (2 ^ machine_wordsize - (a + 1))) with
+          (- a + 2 ^ machine_wordsize) by ring.
+      reflexivity.
+      specialize (Hz a (or_introl eq_refl)); lia.
+      intro; symmetry; apply Z.lt_neq;
+        eapply (weight_positive (uwprops machine_wordsize mw0)).
+      intros; symmetry; apply Z.lt_neq;
+      apply (weight_divides (uwprops machine_wordsize mw0)).
+      intro; symmetry; apply Z.lt_neq;
+        eapply (weight_positive (uwprops machine_wordsize mw0)).
+      intros; symmetry; apply Z.lt_neq;
+        apply (weight_divides (uwprops machine_wordsize mw0)).
+    + intros; apply Hz; right; assumption.
+    + rewrite <- Z.pow_add_r; try apply f_equal; nia. Qed.
+
+Lemma sat_opp_mod2 machine_wordsize n f
+      (mw0 : 0 < machine_wordsize)
+      (Hf : length f = n)
+      (Hz : forall z, In z f -> 0 <= z < 2^machine_wordsize) :
+  sat_mod2 (sat_opp machine_wordsize n f) = sat_mod2 f.
+Proof.
+  rewrite <- !(eval_sat_mod2 machine_wordsize n) by distr_length.
+  rewrite eval_sat_opp; auto.
+  set (x := eval (uweight machine_wordsize) n f).
+  destruct f.
+  - subst. reflexivity.
+  - rewrite <- (Znumtheory.Zmod_div_mod _ (2 ^ (machine_wordsize * Z.of_nat n))).
+    rewrite <- Z.opp_mod2; reflexivity. lia. apply Z.pow_pos_nonneg; nia.
+    apply Zpow_facts.Zpower_divide. simpl in *. nia. Qed.
+
+(*********************************** *)
+(**Properties of twos_complement_opp *)
+(*********************************** *)
+
+Lemma twos_complement_opp_correct m a :
+  (Z.twos_complement_opp m a) = - a mod 2 ^ m.
+Proof.
+  unfold Z.twos_complement_opp.
+  unfold Z.lnot_modulo, Z.lnot.
+  rewrite Zplus_mod_idemp_l.
+  rewrite Z.add_1_r. rewrite Z.succ_pred. reflexivity. Qed.
+
+Lemma twosc_Z_opp a m
+      (Hm : 0 < m) (corner_case : twosc m a <> - 2 ^ (m - 1)) :
+  - twosc m a = twosc m (- a).
+Proof.
+  pose proof twosc_bounds a m Hm.
+
+  assert (0 < 2 ^ (m - 1)) by (apply Z.pow_pos_nonneg; lia).
+  assert (2 ^ m = 2 * 2 ^ (m - 1))
+    by (rewrite Pow.Z.pow_mul_base, Z.sub_simpl_r; lia).
+  assert (0 <= a mod 2 ^ m < 2 ^ m) by (apply Z.mod_pos_bound; lia).
+
+  destruct (dec (a mod 2 ^ m = 2 ^ (m - 1)));
+    destruct (dec (a mod 2 ^ m = 0)); rewrite ?e, ?e0; try lia.
+  - rewrite e, Z.ltb_irrefl in *. lia.
+  - rewrite PullPush.Z.opp_mod_mod, e, Z.mod_0_l by lia.
+    replace (0 <? 2 ^ (m - 1)) with true by (symmetry; apply Z.ltb_lt; lia); reflexivity.
+  - pose proof (mod_less_than_half_iff_not_neg_mod_less _ _ Hm n n0). symmetry in H3.
+    destruct (a mod 2 ^ m <? 2 ^ (m - 1)).
+    + apply negb_true_iff in H3; rewrite H3.
+      apply Z.ltb_ge in H3. rewrite PullPush.Z.opp_mod_mod, Z.mod_opp_small; lia.
+    + apply negb_false_iff in H3; rewrite H3.
+      apply Z.ltb_lt in H3. rewrite PullPush.Z.opp_mod_mod, Z.mod_opp_small; lia. Qed.
+
+Lemma twos_complement_opp_spec m a
+      (Hm : 0 < m)
+      (corner_case : twosc m a <> - 2 ^ (m - 1)) :
+  twosc m (Z.twos_complement_opp m a) = - (twosc m a).
+Proof.
+  unfold Z.twos_complement_opp, Z.lnot_modulo, Z.lnot.
+  rewrite Zplus_mod_idemp_l, Z.add_1_r, Z.succ_pred, twosc_mod by lia. symmetry; apply twosc_Z_opp; lia. Qed.
+
+(************************* *)
+(**Properties of twos_complement_pos *)
+(************************* *)
+
+Lemma twos_complement_pos_spec m a
+      (mw0 : 0 < m)
+      (corner_case : twosc m a <> - 2 ^ (m - 1)) : (* note that this has to be true for Z.twos_complement_pos to work *)
+  Z.twos_complement_pos m a = Z.b2z (0 <? twosc m a).
+Proof.
+  assert (0 < 2 ^ m) by (apply Z.pow_pos_nonneg; lia).
+  assert (0 <= a mod 2 ^ m < 2 ^ m) by (apply Z.mod_pos_bound; lia).
+  assert (2 ^ m = 2 * 2 ^ (m - 1)) by (rewrite Pow.Z.pow_mul_base; ring_simplify (m - 1 + 1); lia).
+
+  unfold Z.twos_complement_pos; cbv [Let_In]; rewrite twos_complement_opp_correct.
+  destruct (a mod 2 ^ m <? 2 ^ (m - 1)) eqn:E; destruct (dec (a mod 2 ^ m = 0)).
+  - rewrite PullPush.Z.opp_mod_mod, e; simpl; rewrite Z.mod_0_l, Z.shiftr_0_l; auto.
+    apply Z.pow_nonzero; lia.
+  - rewrite mod_less_than_half_iff_not_neg_mod_less in E; auto.
+    assert (0 <? a mod 2 ^ m = true) by (apply Z.ltb_lt; lia).
+    rewrite H2, Z.shiftr_div_pow2, Div.Z.div_between_1; try lia; auto.
+    rewrite negb_true_iff, Z.ltb_ge in E.
+    split; try lia.
+    rewrite H1. apply Z.mod_pos_bound; lia. rewrite Z.ltb_lt in E; lia.
+  - rewrite PullPush.Z.opp_mod_mod, e, !Z.mod_0_l, Z.shiftr_0_l; try lia.
+    assert (0 <? 0 - 2 ^ m = false) by (apply Z.ltb_ge; lia). rewrite H2; reflexivity.
+  - rewrite mod_less_than_half_iff_not_neg_mod_less in E; try lia; auto.
+    assert (0 <? a mod 2 ^ m - 2 ^ m = false) by (apply Z.ltb_ge; lia).
+    rewrite H2, Z.shiftr_div_pow2, Z.div_small; try lia; auto.
+    rewrite negb_false_iff, Z.ltb_lt in E. split; try apply Z.mod_pos_bound; lia. Qed.
+
+(****************************************************************************** *)
+(**This section is for the interaction between twosc and integer addition       *)
+(**There are some badly named lemmas. These are just casing on some inequalites *)
+(**of the sum of to numbers under modular reduction.                            *)
+(****************************************************************************** *)
+
+Lemma mod_add a b m
+      (Hm : 0 < m)
+      (Ha : a mod 2 ^ m < (2 ^ (m - 1)))
+      (Hb : b mod 2 ^ m < (2 ^ (m - 1))) :
+  (a + b) mod 2 ^ m = a mod 2 ^ m + b mod 2 ^ m.
+Proof.
+  assert (0 < 2 ^ m) by (apply Z.pow_pos_nonneg; lia).
+  assert (0 <= a mod 2 ^ m) by (apply Z.mod_pos_bound; lia).
+  assert (0 <= b mod 2 ^ m) by (apply Z.mod_pos_bound; lia).
+
+  rewrite <- Zplus_mod_idemp_l, <- Zplus_mod_idemp_r.
+  rewrite Z.mod_small. lia. replace (2 ^ m) with (2 * 2 ^ (m - 1)) at 5. lia.
+  rewrite Pow.Z.pow_mul_base, Z.sub_simpl_r; lia. Qed.
+
+Lemma mod_add2 a b m
+      (Hm : 0 < m)
+      (Ha : a mod 2 ^ m < (2 ^ (m - 1)))
+      (Hb : 2 ^ (m - 1) <= b mod 2 ^ m)
+      (Hsum : (a + b) mod 2 ^ m < 2 ^ (m - 1)) :
+  (a + b) mod 2 ^ m = a mod 2 ^ m + b mod 2 ^ m - 2 ^ m.
+Proof.
+  assert (0 < 2 ^ m) by (apply Z.pow_pos_nonneg; lia).
+  assert (0 <= a mod 2 ^ m < 2 ^ m) by (apply Z.mod_pos_bound; lia).
+  assert (0 <= b mod 2 ^ m < 2 ^ m) by (apply Z.mod_pos_bound; lia).
+  assert (2 ^ m <= a mod 2 ^ m + b mod 2 ^ m < 2 * 2 ^ m).
+  { split; try lia.
+    destruct (dec (2 ^ m <= a mod 2 ^ m + b mod 2 ^ m)); try lia.
+    apply Znot_le_gt in n. rewrite <- Zplus_mod_idemp_l, <- Zplus_mod_idemp_r, Z.mod_small in Hsum; lia. }
+  rewrite <- Zplus_mod_idemp_l, <- Zplus_mod_idemp_r, Modulo.Z.mod_small_1; lia. Qed.
+
+Lemma mod_add3 a b m
+      (Hm : 0 < m)
+      (Ha : a mod 2 ^ m < (2 ^ (m - 1)))
+      (Hb : 2 ^ (m - 1) <= b mod 2 ^ m)
+      (Hsum : 2 ^ (m - 1) <= (a + b) mod 2 ^ m) :
+  (a + b) mod 2 ^ m = a mod 2 ^ m + b mod 2 ^ m.
+Proof.
+  assert (0 < 2 ^ m) by (apply Z.pow_pos_nonneg; lia).
+  assert (0 <= a mod 2 ^ m < 2 ^ m) by (apply Z.mod_pos_bound; lia).
+  assert (0 <= b mod 2 ^ m < 2 ^ m) by (apply Z.mod_pos_bound; lia).
+
+  assert (0 <= a mod 2 ^ m + b mod 2 ^ m < 2 ^ m).
+  split; try lia.
+  destruct (dec (a mod 2 ^ m + b mod 2 ^ m < 2 ^ m)); try lia.
+  apply Znot_lt_ge in n.
+  rewrite <- Zplus_mod_idemp_l, <- Zplus_mod_idemp_r, Modulo.Z.mod_small_1 in Hsum; lia.
+  rewrite <- Zplus_mod_idemp_l, <- Zplus_mod_idemp_r, Z.mod_small; lia. Qed.
+
+Lemma mod_add4 a b m
+      (Hm : 0 < m)
+      (Ha : 2 ^ (m - 1) <= a mod 2 ^ m)
+      (Hb : 2 ^ (m - 1) <= b mod 2 ^ m) :
+  (a + b) mod 2 ^ m = a mod 2 ^ m + b mod 2 ^ m - 2 ^ m.
+Proof.
+  assert (0 < 2 ^ m) by (apply Z.pow_pos_nonneg; lia).
+  assert (0 <= a mod 2 ^ m < 2 ^ m) by (apply Z.mod_pos_bound; lia).
+  assert (0 <= b mod 2 ^ m < 2 ^ m) by (apply Z.mod_pos_bound; lia).
+
+  assert (2 ^ m = 2 * 2 ^ (m - 1))
+    by (rewrite Pow.Z.pow_mul_base, Z.sub_simpl_r; lia).
+
+  rewrite <- Zplus_mod_idemp_l, <- Zplus_mod_idemp_r, Modulo.Z.mod_small_1; lia. Qed.
+
+Lemma twosc_add a b m
+      (Hm : 0 < m)
+      (Ha : - 2 ^ (m - 2) < twosc m a < 2 ^ (m - 2))
+      (Hb : - 2 ^ (m - 2) < twosc m b < 2 ^ (m - 2)) :
+  twosc m (a + b) = twosc m a + twosc m b.
+Proof.
+  destruct (dec (m = 1)).
+  rewrite e in *; replace (2 ^ (1 - 2)) with 0 in * by reflexivity; lia.
+
+  assert (0 < 2 ^ m) by (apply Z.pow_pos_nonneg; lia).
+  assert (2 ^ m = 2 * 2 ^ (m - 1))
+    by (rewrite Pow.Z.pow_mul_base, Z.sub_simpl_r; lia).
+  assert (2 ^ m = 2 * (2 * 2 ^ (m - 2)))
+    by (rewrite !Pow.Z.pow_mul_base; replace (m - 2 + 1 + 1) with m by ring; lia).
+
+  assert (0 <= a mod 2 ^ m < 2 ^ m) by (apply Z.mod_pos_bound; lia).
+  assert (0 <= b mod 2 ^ m < 2 ^ m) by (apply Z.mod_pos_bound; lia).
+
+  destruct ((a + b) mod 2 ^ m <? 2 ^ (m - 1)) eqn:Hsum;
+    destruct (a mod 2 ^ m <? 2 ^ (m - 1)) eqn:Hamod;
+    destruct (b mod 2 ^ m <? 2 ^ (m - 1)) eqn:Hbmod;
+    rewrite ?Z.ltb_lt, ?Z.ltb_ge in *.
+  - apply mod_add; lia.
+  - rewrite Z.add_sub_assoc. apply mod_add2; lia.
+  - rewrite Z.add_comm, <- Z.add_sub_swap.
+    rewrite (Z.add_comm (a mod _)). apply mod_add2; try lia. rewrite Z.add_comm; lia.
+  - assert (2 ^ m <= a mod 2 ^ m + b mod 2 ^ m < 2 * 2 ^ m) by (split; lia).
+    rewrite <- Zplus_mod_idemp_l, <- Zplus_mod_idemp_r, Modulo.Z.mod_small_1 in Hsum; lia.
+  - rewrite <- Zplus_mod_idemp_l, <- Zplus_mod_idemp_r, Z.mod_small in Hsum; lia.
+  - rewrite mod_add3; lia.
+  - rewrite Z.add_comm, mod_add3; try lia. rewrite Z.add_comm; lia.
+  - rewrite mod_add4; lia. Qed.
+
+Lemma mod_add_full a b m
+      (Hm : 0 < m)
+      (Hsum : a mod m + b mod m < m) :
+  (a + b) mod m = a mod m + b mod m.
+Proof.
+  assert (0 <= a mod m < m) by (apply Z.mod_pos_bound; lia).
+  assert (0 <= b mod m < m) by (apply Z.mod_pos_bound; lia).
+  rewrite <- Zplus_mod_idemp_l, <- Zplus_mod_idemp_r, Z.mod_small; lia. Qed.
+
+Lemma twosc_add_full a b m
+      (Hm : 0 < m)
+      (Ha : - 2 ^ (m - 1) <= twosc m a + twosc m b < 2 ^ (m - 1)) :
+  twosc m (a + b) = twosc m a + twosc m b.
+Proof.
+  assert (0 < 2 ^ m) by (apply Z.pow_pos_nonneg; lia).
+  assert (2 ^ m = 2 * 2 ^ (m - 1))
+    by (rewrite Pow.Z.pow_mul_base, Z.sub_simpl_r; lia).
+
+  assert (0 <= a mod 2 ^ m < 2 ^ m) by (apply Z.mod_pos_bound; lia).
+  assert (0 <= b mod 2 ^ m < 2 ^ m) by (apply Z.mod_pos_bound; lia).
+
+  destruct ((a + b) mod 2 ^ m <? 2 ^ (m - 1)) eqn:Hsum;
+    destruct (a mod 2 ^ m <? 2 ^ (m - 1)) eqn:Hamod;
+    destruct (b mod 2 ^ m <? 2 ^ (m - 1)) eqn:Hbmod;
+    rewrite ?Z.ltb_lt, ?Z.ltb_ge in *.
+  - rewrite mod_add_full; lia.
+  - rewrite mod_add2; lia.
+  - rewrite Z.add_comm. rewrite <- Z.add_sub_swap.
+    rewrite (Z.add_comm (a mod _)). apply mod_add2. lia. lia. lia.
+    rewrite Z.add_comm; lia.
+  - assert (2 ^ m <= a mod 2 ^ m + b mod 2 ^ m < 2 * 2 ^ m) by (split; lia).
+    rewrite <- Zplus_mod_idemp_l, <- Zplus_mod_idemp_r, Modulo.Z.mod_small_1 in Hsum; lia.
+  - rewrite <- Zplus_mod_idemp_l, <- Zplus_mod_idemp_r, Z.mod_small in Hsum; lia.
+  - rewrite mod_add3; lia.
+  - rewrite Z.add_comm, mod_add3; try lia. rewrite Z.add_comm; lia.
+  - rewrite mod_add4; lia. Qed.
+
+(********************************************************************* *)
+(**Section for interaction between eval_twosc and saturated operations *)
+(********************************************************************* *)
+
+Lemma eval_twosc_sat_arithmetic_shiftr machine_wordsize n f
+      (mw0 : 0 < machine_wordsize)
+      (n0 : (0 < n)%nat)
+      (Hz : forall z, In z f -> 0 <= z < 2^machine_wordsize)
+      (Hf : length f = n) :
+  eval_twosc machine_wordsize n (sat_arithmetic_shiftr machine_wordsize n f) =
+  (eval_twosc machine_wordsize n f) / 2.
+Proof.
+  assert (0 < Z.of_nat n) by omega. unfold eval_twosc. rewrite eval_sat_arithmetic_shiftr, arithmetic_shiftr_spec; auto; try nia.
+  apply eval_bound; auto. Qed.
+
+Lemma eval_twosc_sat_add machine_wordsize n f g
+      (mw0 : 0 < machine_wordsize)
+      (n0 : (0 < n)%nat)
+      (Hf : length f = n)
+      (Hg : length g = n)
+      (overflow_f : - 2 ^ (machine_wordsize * n - 2) <
+                    twosc (machine_wordsize * n) (eval (uweight machine_wordsize) n f) <
+                    2 ^ (machine_wordsize * n - 2))
+      (overflow_g : - 2 ^ (machine_wordsize * n - 2) <
+                    twosc (machine_wordsize * n) (eval (uweight machine_wordsize) n g) <
+                    2 ^ (machine_wordsize * n - 2)) :
+  eval_twosc machine_wordsize n (sat_add machine_wordsize n f g) =
+  eval_twosc machine_wordsize n f + eval_twosc machine_wordsize n g.
+Proof. assert (0 < Z.of_nat n) by omega. unfold eval_twosc. rewrite eval_sat_add, twosc_mod, twosc_add; nia. Qed.
+
+Lemma eval_twosc_select machine_wordsize n cond f g
+      (Hf : length f = n)
+      (Hg : length g = n) :
+  eval_twosc machine_wordsize n (select cond f g) = if dec (cond = 0)
+                                                    then (eval_twosc machine_wordsize n f)
+                                                    else (eval_twosc machine_wordsize n g).
+Proof. unfold eval_twosc; rewrite eval_select; auto; destruct (dec (cond = 0)); auto. Qed.
+
+Lemma eval_twosc_sat_opp machine_wordsize n f
+      (mw0 : 0 < machine_wordsize)
+      (n0 : (0 < n)%nat)
+      (Hz : forall z, In z f -> 0 <= z < 2^machine_wordsize)
+      (Hf : length f = n)
+      (corner_case : eval_twosc machine_wordsize n f <> - 2 ^ (machine_wordsize * n - 1)):
+  eval_twosc machine_wordsize n (sat_opp machine_wordsize n f) =
+  - eval_twosc machine_wordsize n f.
+Proof. assert (0 < Z.of_nat n) by omega; unfold eval_twosc in *; rewrite eval_sat_opp, twosc_mod, twosc_Z_opp; try nia; tauto. Qed.
+
+Lemma eval_twosc_sat_zero machine_wordsize n
+      (mw0 : 0 < machine_wordsize)
+      (n0 : (0 < n)%nat) :
+  eval_twosc machine_wordsize n (sat_zero n) = 0.
+Proof.
+  unfold eval_twosc; rewrite eval_sat_zero; auto.
+  rewrite Z.mod_0_l by (apply Z.pow_nonzero; nia).
+  assert (0 <? 2 ^ (machine_wordsize * Z.of_nat n - 1) = true) by (apply Z.ltb_lt; apply Z.pow_pos_nonneg; nia).
+  now rewrite H. Qed.
+
+Lemma eval_twosc_sat_mod2 machine_wordsize n f
+      (mw0 : 0 < machine_wordsize)
+      (n0 : (0 < n)%nat)
+      (Hf : length f = n) :
+  (eval_twosc machine_wordsize n f) mod 2 = sat_mod2 f.
+Proof.
+  assert (0 < Z.of_nat n) by omega. unfold eval_twosc. rewrite twosc_mod2, eval_sat_mod2; nia. Qed.
+
+(** ******************************************************************************* *)
+(** This section is for the implementation and correctness of the divstep algorithm *)
+(** ******************************************************************************* *)
+
+Import WordByWordMontgomery.
+Import Positional.
+
+Definition divstep_aux machine_wordsize sat_limbs mont_limbs m (data : Z * (list Z) * (list Z) * (list Z) * (list Z)) :=
+  let r := snd data in
+  let v := snd (fst data) in
+  let g := snd (fst (fst data)) in
+  let f := snd (fst (fst (fst data))) in
+  let d := fst (fst (fst (fst data))) in
+  dlet cond := Z.land (Z.twos_complement_pos machine_wordsize d) (sat_mod2 g) in
+  dlet d' := Z.zselect cond d (Z.twos_complement_opp machine_wordsize d) in
+  dlet f' := select cond f g in
+  dlet g' := select cond g (sat_opp machine_wordsize sat_limbs f) in
+  dlet v' := select cond v r in
+  let v'':= addmod machine_wordsize mont_limbs m v' v' in
+  dlet r' := select cond r (oppmod machine_wordsize mont_limbs m v) in
+  dlet g0 := sat_mod2 g' in
+  let d'' := (d' + 1) mod 2^machine_wordsize in
+  dlet f'' := select g0 (sat_zero sat_limbs) f' in
+  let g'' := sat_arithmetic_shiftr machine_wordsize sat_limbs (sat_add machine_wordsize sat_limbs g' f'') in
+  dlet v''' := select g0 (sat_zero mont_limbs) v' in
+  let r'' := addmod machine_wordsize mont_limbs m r' v''' in
+    (d'',f',g'',v'',r'').
+
+Definition divstep machine_wordsize sat_limbs mont_limbs m d f g v r :=
+  divstep_aux machine_wordsize sat_limbs mont_limbs m (d, f, g, v, r).
+Definition divstep_safe machine_wordsize n :=
+  let sat_limbs := (n + 1)%nat in
+  divstep machine_wordsize sat_limbs n.
+
+Definition divstep_spec d f g :=
+  if (0 <? d) && Z.odd g
+  then (1 - d, g, (g - f) / 2)
+  else (1 + d, f, (g + (g mod 2) * f) / 2 ).
+
+Definition divstep_spec2 m d g v r :=
+  if (0 <? d) && Z.odd g
+  then (2 * r mod m, (r - v) mod m)
+  else (2 * v mod m, (r + (g mod 2) * v) mod m).
+
+Definition divstep_spec_full m d f g v r :=
+  if (0 <? d) && Z.odd g
+  then (1 - d, g, (g - f) / 2, 2 * r mod m, (r - v) mod m)
+  else (1 + d, f, (g + (g mod 2) * f) / 2, 2 * v mod m, (r + (g mod 2) * v) mod m).
+
+Lemma divstep_g machine_wordsize sat_limbs mont_limbs m d f g v r
+      (mw0 : 0 < machine_wordsize)
+      (sat_limbs0 : (0 < sat_limbs)%nat)
+      (fodd : Z.odd (eval_twosc machine_wordsize sat_limbs f) = true)
+      (Hf : length f = sat_limbs)
+      (Hg : length g = sat_limbs)
+      (corner_case : twosc machine_wordsize d <> - 2 ^ (machine_wordsize - 1))
+      (overflow_f : - 2 ^ (machine_wordsize * sat_limbs - 2) <
+                    eval_twosc machine_wordsize sat_limbs f <
+                    2 ^ (machine_wordsize * sat_limbs - 2))
+      (overflow_g : - 2 ^ (machine_wordsize * sat_limbs - 2) <
+                    eval_twosc machine_wordsize sat_limbs g <
+                    2 ^ (machine_wordsize * sat_limbs - 2))
+      (Hf2 : forall z, In z f -> 0 <= z < 2^machine_wordsize)
+      (Hg2 : forall z, In z g -> 0 <= z < 2^machine_wordsize) :
+  let '(d1,f1,g1,v1,r1) := (divstep machine_wordsize sat_limbs mont_limbs m d f g v r) in
+  eval_twosc machine_wordsize sat_limbs g1 =
+  snd (divstep_spec
+         (twosc machine_wordsize d)
+         (eval_twosc machine_wordsize sat_limbs f)
+         (eval_twosc machine_wordsize sat_limbs g)).
+Proof.
+  set (bw := machine_wordsize * Z.of_nat sat_limbs) in *.
+
+  simpl.
+  assert (0 < Z.of_nat sat_limbs) by omega.
+  assert (bw0 : 0 < bw) by nia.
+  assert (bw1 : 1 < bw) by (destruct (dec (bw = 1)); rewrite ?e in *; simpl in *; lia).
+  assert (2 ^ machine_wordsize = 2 * 2 ^ (machine_wordsize - 1))
+    by (rewrite Pow.Z.pow_mul_base, Z.sub_simpl_r; lia).
+  assert (0 < 2 ^ bw) by (apply Z.pow_pos_nonneg; lia).
+  assert (2 ^ (bw - 2) <= 2 ^ (bw - 1)) by (apply Z.pow_le_mono; lia).
+
+  Hint Rewrite length_sat_add length_sat_opp length_select : distr_length.
+
+  rewrite eval_twosc_sat_arithmetic_shiftr; distr_length; autorewrite with distr_length; try nia.
+  rewrite eval_twosc_sat_add; auto; try (autorewrite with distr_length; lia).
+  rewrite !eval_twosc_select; auto; try (autorewrite with distr_length; lia).
+  rewrite eval_twosc_sat_opp; auto; try (autorewrite with distr_length; lia).
+  rewrite select_push; try (autorewrite with distr_length; lia).
+
+  rewrite sat_opp_mod2; auto.
+  unfold divstep_spec.
+  rewrite twos_complement_pos_spec; auto.
+  rewrite <- !(eval_twosc_sat_mod2 machine_wordsize sat_limbs); auto.
+  rewrite !Zmod_odd; auto.
+
+  set (g' := eval_twosc machine_wordsize sat_limbs g) in *.
+  set (f' := eval_twosc machine_wordsize sat_limbs f) in *.
+  assert (corner_case_f : f' <> - 2 ^ (bw - 1)) by
+      (replace (- _) with (- (2 * 2 ^ (bw - 2))); rewrite ?Pow.Z.pow_mul_base; ring_simplify (bw - 2 + 1); nia).
+
+  destruct (0 <? twosc machine_wordsize d);
+    destruct (Z.odd g') eqn:g'_odd; rewrite ?fodd, ?eval_sat_zero; auto.
+  - simpl. rewrite Z.add_comm; reflexivity.
+  - simpl. rewrite eval_twosc_sat_zero; auto.
+  - rewrite Z.mul_1_l. simpl. reflexivity.
+  - simpl. rewrite eval_twosc_sat_zero; auto.
+  - replace (_ * _) with bw by reflexivity. lia.
+  - fold (eval_twosc machine_wordsize sat_limbs
+                     (select (Z.twos_complement_pos machine_wordsize d &' sat_mod2 g) g (sat_opp machine_wordsize sat_limbs f))).
+    rewrite eval_twosc_select; try apply length_sat_opp; auto.
+    destruct (dec (_)); replace (machine_wordsize * _) with bw by reflexivity;
+    try rewrite eval_twosc_sat_opp; auto; replace (machine_wordsize * _) with bw by reflexivity; lia.
+  - fold (eval_twosc machine_wordsize sat_limbs
+                     (select (sat_mod2 (select (Z.twos_complement_pos machine_wordsize d &' sat_mod2 g) g (sat_opp machine_wordsize sat_limbs f)))
+                             (sat_zero sat_limbs) (select (Z.twos_complement_pos machine_wordsize d &' sat_mod2 g) f g))).
+    rewrite eval_twosc_select; try apply length_sat_zero; try apply length_select; auto.
+    destruct (dec (_)); try rewrite eval_twosc_sat_zero; try rewrite eval_twosc_select;
+      replace (machine_wordsize * _) with bw by reflexivity; try lia; destruct (dec (_)); lia.
+  - apply sat_add_bounds; try lia; repeat (rewrite ?length_sat_opp, ?(length_select sat_limbs), ?length_sat_zero; auto). Qed.
+
+Lemma divstep_d machine_wordsize sat_limbs mont_limbs m d f g v r
+      (mw1 : 1 < machine_wordsize)
+      (sat_limbs0 : (0 < sat_limbs)%nat)
+      (Hg : length g = sat_limbs)
+      (overflow_d : - 2 ^ (machine_wordsize - 1) + 1 <
+                    twosc machine_wordsize d <
+                    2 ^ (machine_wordsize - 1) - 1) :
+  let '(d1,f1,g1,v1,r1) := (divstep machine_wordsize sat_limbs mont_limbs m d f g v r) in
+  twosc machine_wordsize d1 =
+  fst (fst (divstep_spec (twosc machine_wordsize d)
+                           (eval_twosc machine_wordsize sat_limbs f)
+                           (eval_twosc machine_wordsize sat_limbs g))).
+Proof.
+  assert (helper0 : 0 < Z.of_nat sat_limbs) by omega.
+  assert (mw0 : 0 < machine_wordsize) by lia.
+  assert (helper : 1 < 2 ^ machine_wordsize) by (apply Zpow_facts.Zpower_gt_1; lia).
+  assert (helper2 : 1 < 2 ^ (machine_wordsize - 1)) by (apply Zpow_facts.Zpower_gt_1; lia).
+  assert (helper3 : 2 ^ machine_wordsize = 2 * 2 ^ (machine_wordsize - 1))
+    by (rewrite Pow.Z.pow_mul_base, Z.sub_simpl_r; lia).
+
+  simpl; unfold divstep_spec.
+  rewrite twos_complement_pos_spec, <- (eval_twosc_sat_mod2 machine_wordsize sat_limbs), Zmod_odd; auto; try nia.
+  fold (eval_twosc machine_wordsize sat_limbs g); set (g' := eval_twosc machine_wordsize sat_limbs g) in *.
+  destruct ((0 <? twosc machine_wordsize d) && (Z.odd g')) eqn:E.
+  - apply andb_prop in E. destruct E; rewrite H, H0. simpl Z.b2z; simpl Z.land; cbv [fst].
+    unfold Z.zselect. simpl (if _ =? _ then _ else _).
+    rewrite twos_complement_opp_correct, twosc_mod, twosc_add_full, twosc_mod, <- twosc_Z_opp, twosc_one; try lia.
+    rewrite twosc_mod, <- twosc_Z_opp, twosc_one; lia.
+  - apply andb_false_iff in E.
+    destruct E; rewrite H;
+      unfold Z.zselect; cbv [fst]; simpl (if _ =? _ then _ else _);
+        [destruct (Z.odd g') | rewrite Z.land_0_r; simpl (if _ =? _ then _ else _)];
+        rewrite twosc_mod, twosc_add_full, twosc_one; try rewrite ?twosc_one; lia. Qed.
+
+Lemma divstep_f machine_wordsize sat_limbs mont_limbs m d f g v r
+      (mw0 : 0 < machine_wordsize)
+      (Hf : length f = sat_limbs)
+      (Hg : length g = sat_limbs)
+      (corner_case : twosc machine_wordsize d <> - 2 ^ (machine_wordsize - 1)) :
+  let '(d1,f1,g1,v1,r1) := (divstep machine_wordsize sat_limbs mont_limbs m d f g v r) in
+  eval_twosc machine_wordsize sat_limbs f1 =
+  snd (fst (divstep_spec (twosc machine_wordsize d)
+                           (eval_twosc machine_wordsize sat_limbs f)
+                           (eval_twosc machine_wordsize sat_limbs g))).
+Proof.
+  destruct sat_limbs. subst.
+  unfold eval_twosc.
+  rewrite !eval0; rewrite Z.mul_0_r.
+  replace (twosc 0 0) with (-1). unfold divstep_spec.
+  destruct (0 <? twosc machine_wordsize d); reflexivity. reflexivity.
+
+  unfold divstep_spec.
+  simpl.
+
+  set (n' := S sat_limbs) in *.
+  assert (0 < n')%nat by apply Nat.lt_0_succ.
+  rewrite eval_twosc_select, twos_complement_pos_spec, <- (eval_twosc_sat_mod2 machine_wordsize n'), Zmod_odd; auto.
+  fold (eval_twosc machine_wordsize n' g).
+  destruct (0 <? twosc machine_wordsize d); destruct (Z.odd (eval_twosc machine_wordsize n' g));
+    try reflexivity; lia. Qed.
+
+Theorem divstep_correct machine_wordsize sat_limbs mont_limbs m d f g v r
+        (mw1 : 1 < machine_wordsize)
+        (sat_limbs0 : (0 < sat_limbs)%nat)
+        (fodd : Z.odd (eval_twosc machine_wordsize sat_limbs f) = true)
+        (Hf : length f = sat_limbs)
+        (Hg : length g = sat_limbs)
+        (overflow_d : - 2 ^ (machine_wordsize - 1) + 1 <
+                    twosc machine_wordsize d <
+                    2 ^ (machine_wordsize - 1) - 1)
+        (overflow_f : - 2 ^ (machine_wordsize * sat_limbs - 2) <
+                      eval_twosc machine_wordsize sat_limbs f <
+                      2 ^ (machine_wordsize * sat_limbs - 2))
+        (overflow_g : - 2 ^ (machine_wordsize * sat_limbs - 2) <
+                      eval_twosc machine_wordsize sat_limbs g <
+                      2 ^ (machine_wordsize * sat_limbs - 2))
+        (Hf2 : forall z, In z f -> 0 <= z < 2^machine_wordsize)
+        (Hg2 : forall z, In z g -> 0 <= z < 2^machine_wordsize) :
+  let '(d1,f1,g1,v1,r1) := (divstep machine_wordsize sat_limbs mont_limbs m d f g v r) in
+  (twosc machine_wordsize d1,
+   eval_twosc machine_wordsize sat_limbs f1,
+   eval_twosc machine_wordsize sat_limbs g1) =
+  divstep_spec (twosc machine_wordsize d)
+               (eval_twosc machine_wordsize sat_limbs f)
+               (eval_twosc machine_wordsize sat_limbs g).
+Proof.
+  assert (0 < machine_wordsize) by lia.
+  apply injective_projections.
+  apply injective_projections.
+  rewrite <- (divstep_d _ _ mont_limbs m _ _ _ v r); auto.
+  rewrite <- (divstep_f _ _ mont_limbs m _ _ _ v r); auto; lia.
+  rewrite <- (divstep_g _ _ mont_limbs m _ _ _ v r); auto; lia. Qed.
+
+Lemma divstep_v machine_wordsize sat_limbs mont_limbs m (r' : Z) m' d f g v r
+      (fodd : Z.odd (eval_twosc machine_wordsize sat_limbs f) = true)
+
+      (r'_correct : (2 ^ machine_wordsize * r') mod m = 1)
+      (m'_correct : (m * m') mod 2 ^ machine_wordsize = -1 mod 2 ^ machine_wordsize)
+      (m_big : 1 < m)
+      (m_small : m < (2 ^ machine_wordsize) ^ Z.of_nat mont_limbs)
+      (Hv2 : valid machine_wordsize mont_limbs m v)
+      (Hr2 : valid machine_wordsize mont_limbs m r)
+      (mw0 : 0 < machine_wordsize)
+      (sat_limbs0 : (0 < sat_limbs)%nat)
+      (mont_limbs0 : (0 < mont_limbs)%nat)
+      (Hv : length v = mont_limbs)
+      (Hr : length r = mont_limbs)
+      (Hg : length g = sat_limbs)
+      (overflow_d : - 2 ^ (machine_wordsize - 1) + 1 <
+                    twosc machine_wordsize d <
+                    2 ^ (machine_wordsize - 1) - 1) :
+  let '(d1,f1,g1,v1,r1) := (divstep machine_wordsize sat_limbs mont_limbs m d f g v r) in
+  @WordByWordMontgomery.eval machine_wordsize mont_limbs
+                        (from_montgomerymod machine_wordsize mont_limbs m m' v1) mod m =
+  fst (divstep_spec2 m (twosc machine_wordsize d)
+                (eval_twosc machine_wordsize sat_limbs g)
+                (@WordByWordMontgomery.eval machine_wordsize mont_limbs
+                                       (from_montgomerymod machine_wordsize mont_limbs m m' v))
+                (@WordByWordMontgomery.eval machine_wordsize mont_limbs
+                                       (from_montgomerymod machine_wordsize mont_limbs m m' r))).
+Proof.
+  assert (sat_limbs <> 0%nat) by lia.
+  assert (mont_limbs <> 0%nat) by lia.
+  simpl.
+  rewrite twos_complement_pos_spec, <- (eval_twosc_sat_mod2 machine_wordsize sat_limbs) by lia.
+  rewrite Zmod_odd, (select_eq (uweight machine_wordsize) _ mont_limbs); auto.
+  unfold divstep_spec2.
+  destruct (0 <? twosc machine_wordsize d);
+    destruct (Z.odd (eval_twosc machine_wordsize sat_limbs g));
+    rewrite ?(eval_addmod _ _ _ r'), ?Z.add_diag; auto. Qed.
+
+Lemma nonzero_zero n :
+  nonzeromod (sat_zero n) = 0.
+Proof. unfold nonzero, sat_zero; induction n; auto. Qed.
+
+Lemma zero_valid machine_wordsize n m
+      (mw0 : 0 < machine_wordsize)
+      (m0 : 0 < m) :
+  valid machine_wordsize n m (sat_zero n).
+Proof.
+  unfold valid, small, WordByWordMontgomery.eval.
+  rewrite eval_sat_zero, partition_0; try split; auto; try lia. Qed.
+
+Lemma divstep_r machine_wordsize sat_limbs mont_limbs m (r' : Z) m' d f g v r
+      (fodd : Z.odd (eval_twosc machine_wordsize sat_limbs f) = true)
+      (r'_correct : (2 ^ machine_wordsize * r') mod m = 1)
+      (m'_correct : (m * m') mod 2 ^ machine_wordsize = -1 mod 2 ^ machine_wordsize)
+      (m_big : 1 < m)
+      (m_small : m < (2 ^ machine_wordsize) ^ Z.of_nat mont_limbs)
+      (Hv2 : valid machine_wordsize mont_limbs m v)
+      (Hr2 : valid machine_wordsize mont_limbs m r)
+      (mw0 : 0 < machine_wordsize)
+      (sat_limbs0 : (0 < sat_limbs)%nat)
+      (mont_limbs0 : (0 < mont_limbs)%nat)
+      (Hv : length v = mont_limbs)
+      (Hr : length r = mont_limbs)
+      (Hf : length f = sat_limbs)
+      (Hg : length g = sat_limbs)
+      (overflow_d : - 2 ^ (machine_wordsize - 1) + 1 <
+                    twosc machine_wordsize d <
+                    2 ^ (machine_wordsize - 1) - 1)
+      (Hf2 : forall z, In z f -> 0 <= z < 2^machine_wordsize) :
+  let '(d1,f1,g1,v1,r1) := (divstep machine_wordsize sat_limbs mont_limbs m d f g v r) in
+  @WordByWordMontgomery.eval machine_wordsize mont_limbs
+                        (from_montgomerymod machine_wordsize mont_limbs m m' r1) mod m =
+  snd (divstep_spec2 m (twosc machine_wordsize d)
+                (eval_twosc machine_wordsize sat_limbs g)
+                (@WordByWordMontgomery.eval machine_wordsize mont_limbs
+                                       (from_montgomerymod machine_wordsize mont_limbs m m' v))
+                (@WordByWordMontgomery.eval machine_wordsize mont_limbs
+                                       (from_montgomerymod machine_wordsize mont_limbs m m' r))).
+Proof.
+  Arguments Z.mul : simpl never.
+  assert (sat_limbs0' : (sat_limbs <> 0%nat)) by lia.
+  assert (mont_limbs0' : mont_limbs <> 0%nat) by lia.
+  unfold divstep_spec2.
+  pose proof (oppmod_correct machine_wordsize mont_limbs m r' m' r'_correct m'_correct mw0 m_big (ltac:(lia)) m_small) as H.
+  destruct H as [H1 H2].
+  assert (zero_valid : valid machine_wordsize mont_limbs m (sat_zero mont_limbs)) by (apply zero_valid; lia).
+  pose proof (nonzero_zero mont_limbs) as H3.
+  rewrite (nonzeromod_correct machine_wordsize mont_limbs m r' m') in H3; try apply zero_valid; try lia; auto.
+
+  simpl.
+  rewrite select_push; rewrite ?length_sat_opp; auto.
+  rewrite sat_opp_mod2; auto.
+  rewrite twos_complement_pos_spec, <- !(eval_twosc_sat_mod2 machine_wordsize sat_limbs); try lia.
+  rewrite !Zmod_odd, !(select_eq (uweight machine_wordsize) _ mont_limbs), fodd;
+    try apply length_select; auto.
+  destruct (0 <? twosc machine_wordsize d);
+    destruct (Z.odd (eval_twosc machine_wordsize sat_limbs g)); simpl.
+  - rewrite (eval_addmod _ _ _ r'); auto.
+    rewrite <- Zplus_mod_idemp_l; auto.
+    rewrite (eval_oppmod _ _ _ r'); auto.
+    rewrite Zplus_mod_idemp_l; auto.
+    rewrite Z.add_comm; unfold Z.sub; auto.
+  - rewrite (eval_addmod _ _ _ r'); auto.
+    rewrite <- Zplus_mod_idemp_r; auto.
+    rewrite H3.
+    rewrite Z.mul_0_l, Z.add_0_r; auto.
+  - rewrite (eval_addmod _ _ _ r'); auto.
+    rewrite Z.mul_1_l; auto.
+  - rewrite (eval_addmod _ _ _ r'); auto.
+    rewrite <- Zplus_mod_idemp_r; auto.
+    rewrite H3.
+    rewrite Z.mul_0_l, Z.add_0_r; auto.
+  - apply length_sat_zero.
+  - unfold oppmod, WordByWordMontgomery.opp,
+    WordByWordMontgomery.sub, Rows.sub_then_maybe_add, Rows.add.
+    destruct (Rows.sub (uweight machine_wordsize) mont_limbs (zeros mont_limbs)) eqn:E.
+    destruct (Rows.flatten (uweight machine_wordsize) mont_limbs
+                           [l; zselect (2 ^ machine_wordsize - 1) (- z) (Partition.partition (uweight machine_wordsize) mont_limbs m)]) eqn:E2.
+    simpl.
+    inversion E; subst.
+    inversion E2.
+    apply Rows.length_sum_rows.
+    apply (uwprops machine_wordsize mw0).
+    apply Rows.length_sum_rows.
+    apply (uwprops machine_wordsize mw0).
+    apply length_zeros.
+    apply map_length.
+    rewrite length_zselect.
+    apply length_partition. Qed.
+
+Lemma divstep_spec_divstep_spec_full_d m d f g v r :
+  fst (fst (divstep_spec d f g)) = fst (fst (fst (fst (divstep_spec_full m d f g v r)))).
+Proof. unfold divstep_spec, divstep_spec_full.
+       destruct ((0 <? d) && Z.odd g); reflexivity. Qed.
+
+Lemma divstep_spec_divstep_spec_full_f m d f g v r :
+  snd (fst (divstep_spec d f g)) = snd (fst (fst (fst (divstep_spec_full m d f g v r)))).
+Proof. unfold divstep_spec, divstep_spec_full.
+       destruct ((0 <? d) && Z.odd g); reflexivity. Qed.
+
+Lemma divstep_spec_divstep_spec_full_g m d f g v r :
+  snd (divstep_spec d f g) = snd (fst (fst (divstep_spec_full m d f g v r))).
+Proof. unfold divstep_spec, divstep_spec_full.
+       destruct ((0 <? d) && Z.odd g); reflexivity. Qed.
+
+Lemma divstep_spec2_divstep_spec_full_v m d f g v r :
+  fst (divstep_spec2 m d g v r) = snd (fst (divstep_spec_full m d f g v r)).
+Proof. unfold divstep_spec2, divstep_spec_full.
+       destruct ((0 <? d) && Z.odd g); reflexivity. Qed.
+
+Lemma divstep_spec2_divstep_spec_full_r m d f g v r :
+  snd (divstep_spec2 m d g v r) = snd (divstep_spec_full m d f g v r).
+Proof. unfold divstep_spec2, divstep_spec_full.
+       destruct ((0 <? d) && Z.odd g); reflexivity. Qed.
+
+Theorem divstep_correct_full machine_wordsize sat_limbs mont_limbs m r' m' d f g v r
+      (fodd : Z.odd (eval_twosc machine_wordsize sat_limbs f) = true)
+      (r'_correct : (2 ^ machine_wordsize * r') mod m = 1)
+      (m'_correct : (m * m') mod 2 ^ machine_wordsize = -1 mod 2 ^ machine_wordsize)
+      (m_big : 1 < m)
+      (m_small : m < (2 ^ machine_wordsize) ^ Z.of_nat mont_limbs)
+      (mw1 : 1 < machine_wordsize)
+      (sat_limbs0 : (0 < sat_limbs)%nat)
+      (mont_limbs0 : (0 < mont_limbs)%nat)
+      (Hv : length v = mont_limbs)
+      (Hr : length r = mont_limbs)
+      (Hf : length f = sat_limbs)
+      (Hg : length g = sat_limbs)
+      (overflow_d : - 2 ^ (machine_wordsize - 1) + 1 <
+                    twosc machine_wordsize d <
+                    2 ^ (machine_wordsize - 1) - 1)
+      (overflow_f : - 2 ^ (machine_wordsize * sat_limbs - 2) <
+                    eval_twosc machine_wordsize sat_limbs f <
+                    2 ^ (machine_wordsize * sat_limbs - 2))
+      (overflow_g : - 2 ^ (machine_wordsize * sat_limbs - 2) <
+                    eval_twosc machine_wordsize sat_limbs g <
+                    2 ^ (machine_wordsize * sat_limbs - 2))
+      (Hf2 : forall z, In z f -> 0 <= z < 2^machine_wordsize)
+      (Hg2 : forall z, In z g -> 0 <= z < 2^machine_wordsize)
+      (Hv2 : valid machine_wordsize mont_limbs m v)
+      (Hr2 : valid machine_wordsize mont_limbs m r) :
+  let '(d1,f1,g1,v1,r1) := (divstep machine_wordsize sat_limbs mont_limbs m d f g v r) in
+    (twosc machine_wordsize d1,
+     eval_twosc machine_wordsize sat_limbs f1,
+     eval_twosc machine_wordsize sat_limbs g1,
+     @WordByWordMontgomery.eval machine_wordsize mont_limbs (from_montgomerymod machine_wordsize mont_limbs m m' v1) mod m,
+     @WordByWordMontgomery.eval machine_wordsize mont_limbs (from_montgomerymod machine_wordsize mont_limbs m m' r1) mod m) =
+    divstep_spec_full m (twosc machine_wordsize d)
+                      (eval_twosc machine_wordsize sat_limbs f)
+                      (eval_twosc machine_wordsize sat_limbs g)
+                      (@WordByWordMontgomery.eval machine_wordsize mont_limbs (from_montgomerymod machine_wordsize mont_limbs m m' v))
+                      (@WordByWordMontgomery.eval machine_wordsize mont_limbs (from_montgomerymod machine_wordsize mont_limbs m m' r)).
+Proof.
+  assert (0 < machine_wordsize) by lia.
+  repeat apply injective_projections.
+  rewrite <- divstep_spec_divstep_spec_full_d, <- (divstep_d _ _ mont_limbs m _ _ _ v r); auto.
+  rewrite <- divstep_spec_divstep_spec_full_f, <- (divstep_f _ _ mont_limbs m _ _ _ v r); auto; lia.
+  rewrite <- divstep_spec_divstep_spec_full_g, <- (divstep_g _ _ mont_limbs m _ _ _ v r); auto; lia.
+  rewrite <- divstep_spec2_divstep_spec_full_v;
+    rewrite <- (divstep_v _ _ _ _ r' _ _ f _ _ _); auto.
+  rewrite <- divstep_spec2_divstep_spec_full_r;
+    rewrite <- (divstep_r _ _ _ _ r' _ _ f _ _ _); auto. Qed.
