src/PushButtonSynthesis/WordByWordMontgomeryReificationCache.v
@@ -274,9 +274,10 @@ Local Opaque reified_%s_gen. (* needed for making [autorewrite] not take a very 
          SuchThat (is_reification_of reified_one_gen onemod)
          As reified_one_gen_correct.
   Proof.
-    (* Time cache_reify (). *)
+    Time cache_reify ().
+    (* Note that the following speed up breaks compilation of binaries /benjamin *)
     (* we do something faster *)
-    Time cache_reify_faster_1arg ().
+    (* Time cache_reify_faster_1arg ().  *)
   Time Qed.
   Hint Extern 1 (_ = _) => apply_cached_reification onemod (proj1 reified_one_gen_correct) : reify_cache_gen.
   Hint Immediate (proj2 reified_one_gen_correct) : wf_gen_cache.
