src/Util/ZUtil/Land.v
@@ -1,8 +1,10 @@
 Require Import Coq.ZArith.ZArith.
 Require Import Coq.micromega.Lia.
+Require Import Coq.Bool.Bool.
 Require Import Crypto.Util.ZUtil.Notations.
 Require Import Crypto.Util.ZUtil.Definitions.
 Require Import Crypto.Util.ZUtil.Hints.Core.
+Require Import Crypto.Util.ZUtil.Testbit.
 Local Open Scope bool_scope. Local Open Scope Z_scope.
 
 Module Z.
@@ -55,6 +57,37 @@ Module Z.
       by auto with zarith.
     rewrite Z.land_ones_low; auto with zarith.
   Qed.
+  
+  Lemma land_pow2_testbit a b :
+  a &' 2^b = if Z.testbit a b then 2^b else 0.
+  Proof.
+    apply Z.bits_inj_iff; red; intros; rewrite Z.land_spec.
+    destruct (Z.testbit a b) eqn:E.
+    - destruct (Z.eqb_spec b n); subst.
+      + now rewrite E, andb_true_l.
+      + now rewrite Z.pow2_bits_false, andb_false_r.
+    - rewrite Z.testbit_0_l; destruct (Z.eqb_spec b n); subst.
+      + now rewrite E, andb_false_l.
+      + now rewrite Z.pow2_bits_false, andb_false_r. Qed.
+
+  Lemma land_pow2_small a b
+        (Ha : 0 <= a < 2^b) :
+    a &' 2^b = 0.
+  Proof. now rewrite land_pow2_testbit, Testbit.Z.bits_above_pow2. Qed.
+
+  Lemma land_pow2_small_neg a b
+        (Ha : - 2^b <= a < 0)
+        (Hb : 0 < b) :
+    a &' 2^b = 2^b.
+  Proof. now rewrite land_pow2_testbit, Testbit.Z.testbit_small_neg. Qed.
+
+  Lemma land_div2 a b (Ha : 0 <= a < 2^(b + 1))  :
+    a / 2 &' 2^b = 0.
+  Proof.
+    destruct (Z.ltb_spec b 0).
+    - now rewrite Pow.Z.base_pow_neg, Z.land_0_r.
+    - rewrite land_pow2_testbit, Z.div2_bits, Testbit.Z.bits_above_pow2; 
+      try (replace (Z.succ b) with (b + 1); nia). Qed.
 
   Lemma land_pow2 x n :
     0 <= n ->
