src/Util/ZUtil/Modulo.v
@@ -345,6 +345,12 @@ Module Z.
   Proof. intros; rewrite (mod_small_n 1) by lia; lia. Qed.
   Hint Rewrite mod_small_1 using zutil_arith : zsimplify.
 
+  Lemma mod_opp_small a m : 0 < a <= m -> (-a) mod m = m - a.
+  Proof. intros; symmetry; apply Zmod_unique with (-1); lia. Qed.
+
+  Lemma mod_neg_small a m : -m <= a < 0 -> a mod m = m + a.
+  Proof. intros; symmetry; apply Zmod_unique with (-1); lia. Qed.
+
   Lemma mod_small_n_if n a b : 0 <= n -> b <> 0 -> n * b <= a < (2 + n) * b -> a mod b = a - (if (1 + n) * b <=? a then (1 + n) else n) * b.
   Proof. intros; erewrite Zmod_eq_full, Z.div_between_if by eassumption; autorewrite with zsimplify_const. reflexivity. Qed.
 
@@ -382,6 +388,9 @@ Module Z.
     reflexivity.
   Qed.
 
+  Lemma opp_mod2 a : a mod 2 = - a mod 2.
+  Proof. rewrite !Zmod_odd, Z.odd_opp; reflexivity. Qed.
+  
   Lemma mod_pow_same_base_larger a b n m :
     0 <= n < m -> 0 < b ->
     (a mod (b^n)) mod (b^m) = a mod b^n.
