inversion-c/readme.txt
@@ -1,0 +1,11 @@
+inversion.c contains an implementation of inversion modulo p. To
+change the prime modulus (or wordsize), compile montgomery_inversion.v
+in src/ExtractionOCaml/, compile the extracted .ml and call the binary
+as, e.g.,
+
+./montgomery_inversion test '2^414 - 17' 64 > ../../inversion-c/montgomery_inversion.c
+
+where you change '2^414 - 17' with your desired prime and 64 with your
+desired wordsize. You also need to change a few values in inversion.c
+(see the file). Note that if you use a curve description different
+from 'test' then you have to change inversion.c accordingly.
